Finish IntOrBool

examples/steel/arraystructs/IntOrBool.fsti
@@ -13,7 +13,7 @@ module A = Steel.Effect.Atomic
 
 type int_or_bool_case = | I | B
 
-val int_or_bool: Type
+val int_or_bool: Type0
 
 /// PCM for node:
 
@@ -22,8 +22,10 @@ val int_or_bool_pcm: pcm int_or_bool
 /// (mk_int i) represents (union int_or_bool){.i = i}
 /// (mk_bool b) represents (union int_or_bool){.b = b}
 
-val mk_int (i: Ghost.erased (pod int)): Ghost.erased int_or_bool
-val mk_bool (i: Ghost.erased (pod bool)): Ghost.erased int_or_bool
+let nonunit (p: pcm 'a) = x:'a{~ (x == one p)}
+
+val mk_int (i: Ghost.erased (nonunit (pod_pcm int))): Ghost.erased int_or_bool
+val mk_bool (b: Ghost.erased (nonunit (pod_pcm bool))): Ghost.erased int_or_bool
 
 /// Connections for cases
 
@@ -32,39 +34,52 @@ val _b : int_or_bool_pcm `connection` pod_pcm bool
 
 /// Getting the case of a union in GTot
 
-// Construct using strong LEM
-val case_of_int_or_bool (u: Ghost.erased int_or_bool): GTot (option int_or_bool_case)
+val case_of_int_or_bool (u: Ghost.erased int_or_bool):
+  GTot (k:option int_or_bool_case{
+    match k with
+    | Some I -> exists i. u == mk_int i
+    | Some B -> exists b. u == mk_bool b
+    | None -> Ghost.reveal u == one int_or_bool_pcm
+  })
 
-val case_of_int_or_bool_int (i: Ghost.erased (pod int))
+val case_of_int_or_bool_int (i: Ghost.erased (nonunit (pod_pcm int)))
 : Lemma (case_of_int_or_bool (mk_int i) == Some I) [SMTPat (mk_int i)]
 
-val case_of_int_or_bool_bool (b: Ghost.erased (pod bool))
+val case_of_int_or_bool_bool (b: Ghost.erased (nonunit (pod_pcm bool)))
 : Lemma (case_of_int_or_bool (mk_bool b) == Some B) [SMTPat (mk_bool b)]
 
 val case_of_int_or_bool_one
 : squash (case_of_int_or_bool (one int_or_bool_pcm) == None)
 
+val mk_int_exclusive (i: Ghost.erased (nonunit (pod_pcm int)))
+: Lemma (requires exclusive (pod_pcm int) i) (ensures exclusive int_or_bool_pcm (mk_int i))
+  [SMTPat (exclusive (pod_pcm int) i)]
+
+val mk_bool_exclusive (b: Ghost.erased (nonunit (pod_pcm bool)))
+: Lemma (requires exclusive (pod_pcm bool) b) (ensures exclusive int_or_bool_pcm (mk_bool b))
+  [SMTPat (exclusive (pod_pcm bool) b)]
+
 /// Taking pointers to the i and b cases of an int_or_bool
 
-val addr_of_i (#i: Ghost.erased (pod int)) (p: ref 'a int_or_bool_pcm)
+val addr_of_i (#i: Ghost.erased (nonunit (pod_pcm int))) (p: ref 'a int_or_bool_pcm)
 : SteelT (q:ref 'a (pod_pcm int){q == ref_focus p _i})
     (p `pts_to` mk_int i)
-    (fun q -> q `pts_to` i)
+    (fun q -> q `pts_to` Ghost.reveal i)
 
-val unaddr_of_i (#i: Ghost.erased (pod int)) (#opened: M.inames)
+val unaddr_of_i (#i: Ghost.erased (nonunit (pod_pcm int))) (#opened: M.inames)
   (p: ref 'a int_or_bool_pcm)
   (q: ref 'a (pod_pcm int){q == ref_focus p _i})
-: A.SteelGhostT unit opened (q `pts_to` i) (fun _ -> p `pts_to` mk_int i)
+: A.SteelGhostT unit opened (q `pts_to` Ghost.reveal i) (fun _ -> p `pts_to` mk_int i)
 
-val addr_of_b (#b: Ghost.erased (pod bool)) (p: ref 'a int_or_bool_pcm)
+val addr_of_b (#b: Ghost.erased (nonunit (pod_pcm bool))) (p: ref 'a int_or_bool_pcm)
 : SteelT (q:ref 'a (pod_pcm bool){q == ref_focus p _b})
     (p `pts_to` mk_bool b)
-    (fun q -> q `pts_to` b)
+    (fun q -> q `pts_to` Ghost.reveal b)
 
-val unaddr_of_b (#b: Ghost.erased (pod bool)) (#opened: M.inames)
+val unaddr_of_b (#b: Ghost.erased (nonunit (pod_pcm bool))) (#opened: M.inames)
   (p: ref 'a int_or_bool_pcm)
   (q: ref 'a (pod_pcm bool){q == ref_focus p _b})
-: A.SteelGhostT unit opened (q `pts_to` b) (fun _ -> p `pts_to` mk_bool b)
+: A.SteelGhostT unit opened (q `pts_to` Ghost.reveal b) (fun _ -> p `pts_to` mk_bool b)
 
 /// Switching the case
 
@@ -72,14 +87,14 @@ val switch_to_int (#u: Ghost.erased int_or_bool)
   (p: ref 'a int_or_bool_pcm) (i: int)
 : Steel unit
     (p `pts_to` u)
-    (fun _ -> p `pts_to` mk_int (some i))
-    (requires fun _ -> Some? (case_of_int_or_bool u))
-    (requires fun _ _ _ -> True)
+    (fun _ -> p `pts_to` mk_int (Ghost.hide (Ghost.reveal (some i))))
+    (requires fun _ -> Some? (case_of_int_or_bool u) /\ exclusive int_or_bool_pcm u)
+    (ensures fun _ _ _ -> True)
 
 val switch_to_bool (#u: Ghost.erased int_or_bool)
   (p: ref 'a int_or_bool_pcm) (b: bool)
 : Steel unit
     (p `pts_to` u)
-    (fun _ -> p `pts_to` mk_bool (some b))
-    (requires fun _ -> Some? (case_of_int_or_bool u))
-    (requires fun _ _ _ -> True)
+    (fun _ -> p `pts_to` mk_bool (Ghost.hide (Ghost.reveal (some b))))
+    (requires fun _ -> Some? (case_of_int_or_bool u) /\ exclusive int_or_bool_pcm u)
+    (ensures fun _ _ _ -> True)
